#188 sbElem.thy and changed medium input to use sbElem

automat/CaseStudy/PreludeMed.thy
@@ -47,23 +47,6 @@ fun medMessageTransform :: "'a medMessage tsyn \<Rightarrow> 'a tsyn" where
 
 
 
-
-section\<open>General\<close>
-(* Move this somewhere else... *)
-lift_definition tsynNullElem :: "channel set \<Rightarrow> 'a::message tsyn sbElem" is
-"\<lambda>cs. (\<lambda>c. (c\<in>cs) \<leadsto> -)"
- unfolding sbElemWell_def
-  unfolding usclOkay_stream_def
-  unfolding ctype_tsyn_def
-  by simp
-
-lift_definition sbElem2SB::"'a::message sbElem \<Rightarrow> 'a SB" is
-"\<lambda> elem. (\<lambda>c. (c\<in>dom (Rep_sbElem elem)) \<leadsto> \<up>(Rep_sbElem elem)\<rightharpoonup>c)"
-  unfolding ubWell_def
-  unfolding usclOkay_stream_def
-  apply simp
-  using sbElemWellI Rep_sbElem by blast
-
 section \<open>MedIn\<close>
 
   subsection\<open>Definitions\<close>
@@ -72,22 +55,30 @@ section \<open>MedIn\<close>
 definition medInDom :: "channel set" where
 "medInDom = { \<C> ''in'' }"
 
-lift_definition medInMsg :: "'a \<Rightarrow> 'a medMessage tsyn SB" is
-"\<lambda>x. [ \<C> ''in'' \<mapsto> \<up>(Msg (medData x))]"
-  unfolding ubWell_def
+
+lift_definition medInMsgElem :: "'a \<Rightarrow> 'a medMessage tsyn sbElem" is
+"\<lambda>x. [ (\<C> ''in'') \<mapsto> (Msg (medData x))]"
+  unfolding sbElemWell_def
   unfolding usclOkay_stream_def
   unfolding ctype_tsyn_def
   by simp
 
-fun medIn ::"'a tsyn \<Rightarrow> 'a medMessage tsyn SB" where
-"medIn (Msg m) = medInMsg m" |
-"medIn   -     = tsynbNull  (\<C> ''in'')"
+fun medInElem ::"'a tsyn \<Rightarrow> 'a medMessage tsyn sbElem" where
+"medInElem (Msg m) = medInMsgElem m" |
+"medInElem   -     = sbeNull medInDom"
+declare medInElem.simps[simp del]
 
+fun medIn ::"'a tsyn \<Rightarrow> 'a medMessage tsyn SB" where
+"medIn m = sbe2SB(medInElem m)"
 
   subsection\<open>Lemma\<close>
 
-lemma medinmsg_dom[simp]: "ubDom\<cdot>(medInMsg a) = medInDom"
-  by(simp add: ubdom_insert medInMsg.rep_eq medInDom_def)
+lemma medinmsgelem_dom[simp]: "sbeDom (medInMsgElem a) = medInDom"
+  by(simp add: sbeDom_def medInMsgElem.rep_eq medInDom_def)
+
+lemma medinelem_dom[simp]: "sbeDom (medInElem a) = medInDom"
+  apply(cases a)
+  by (auto simp add: medInElem.simps)
 
 lemma medin_dom[simp]: "ubDom\<cdot>(medIn a) = medInDom"
   by(cases a, simp_all add: medInDom_def)
@@ -115,30 +106,23 @@ lift_definition medOutMsgElem :: "'a \<Rightarrow> 'a medMessage tsyn sbElem" is
 
 fun medOutElem ::"'a tsyn \<Rightarrow> 'a medMessage tsyn sbElem" where
 "medOutElem (Msg m) = medOutMsgElem m" |
-"medOutElem   -     = tsynNullElem medOutDom"
-
-
-
-lift_definition medOutMsg :: "'a \<Rightarrow> 'a medMessage tsyn SB" is
-"\<lambda>x. [ \<C> ''out'' \<mapsto> \<up>(Msg (medData x))]"
-  unfolding ubWell_def
-  unfolding usclOkay_stream_def
-  unfolding ctype_tsyn_def
-  by simp
+"medOutElem   -     = sbeNull medOutDom"
+declare medOutElem.simps[simp del]
 
 fun medOut ::"'a tsyn \<Rightarrow> 'a medMessage tsyn SB" where
-"medOut (Msg m) = medOutMsg m" |
-"medOut   -     = tsynbNull  (\<C> ''out'')"
-
-
+"medOut m = sbe2SB(medOutElem m)"
 
   subsection\<open>Lemma\<close>
 
-lemma medoutmsg_dom[simp]: "ubDom\<cdot>(medOutMsg a) = medOutDom"
-  by(simp add: ubdom_insert medOutMsg.rep_eq medOutDom_def)
+lemma medoutmsgelem_dom[simp]: "sbeDom (medOutMsgElem a) = medOutDom"
+  by(simp add: sbeDom_def medOutMsgElem.rep_eq medOutDom_def)
+
+lemma medoutelem_dom[simp]: "sbeDom (medOutElem a) = medOutDom"
+  apply(cases a)
+  by (auto simp add: medOutElem.simps)
 
 lemma medout_dom[simp]: "ubDom\<cdot>(medOut a) = medOutDom"
-  by(cases a, simp_all add: medOutDom_def)
+  by(cases a, simp_all add: medInDom_def)
 
 
 end
